wip: fix most of UntypedComp; need to prove eliminate

src/UntypedComp.v
@@ -2,6 +2,9 @@ Require Import List Arith Omega.
 Import ListNotations.
 
 Require Import StructTact.StructTactics.
+Require Import Utopia.
+Require Import Program.
+
 
 Require SourceLang.
 Require Untyped.
@@ -9,34 +12,17 @@ Require Untyped.
 Module S := SourceLang.
 Module U := Untyped.
 
-Definition type_name (tn : S.type_name) : U.type_name :=
-  match tn with
-  | S.Bool    => U.Tbool
-  | S.Nat     => U.Tnat
-  | S.ListNat => U.Tlist_nat
-  end.
-
-Definition constr_name {l ty} (c : S.constr l ty) : U.constr_name :=
-  match c with
-  | S.CTrue  => U.Ctrue
-  | S.CFalse => U.Cfalse
-  | S.CZero  => U.CO
-  | S.CSucc  => U.CS
-  | S.CNil   => U.Cnil
-  | S.CCons  => U.Ccons
-  end.
-
 Fixpoint member {A} {ty : A} {l} (m : S.member ty l) : nat :=
   match m with
   | S.Here => 0
   | S.There m' => S (member m')
   end.
 
-Definition elim_to_type_name {l cases target} (e : S.elim l cases target) : U.type_name :=
+Definition elim_to_type_name {l cases target} (e : S.elim l cases target) : type_name :=
   match e with
-  | S.EBool _ => U.Tbool
-  | S.ENat _ => U.Tnat
-  | S.EListNat _ => U.Tlist_nat
+  | S.EBool _ => Tbool
+  | S.ENat _ => Tnat
+  | S.EListNat _ => Tlist_nat
   end.
 
 Definition compile {l ty} (e : S.expr l ty) : U.expr :=
@@ -48,11 +34,11 @@ Definition compile {l ty} (e : S.expr l ty) : U.expr :=
           end
       in
       match e with
-      | S.Var v               => U.Var (member v)
-      | S.Lam b               => U.Lam (go b)
-      | S.App e1 e2           => U.App (go e1) (go e2)
-      | S.Constr c args       => U.Constr (constr_name c) (go_hlist args)
-      | S.Elim e cases target => U.Elim (elim_to_type_name e) (go_hlist cases) (go target)
+      | S.Var v                   => U.Var (member v)
+      | S.Lam b                   => U.Lam (go b)
+      | S.App e1 e2               => U.App (go e1) (go e2)
+      | @S.Constr  _ _ _ c _ args => U.Constr c (go_hlist args)
+      | S.Elim e cases target     => U.Elim (elim_to_type_name e) (go_hlist cases) (go target)
       end
   in go e.
 
@@ -62,7 +48,6 @@ Fixpoint hmap_simple {A} {B : A -> Type} {C l} (f : forall a, B a -> C) (h : S.h
   | S.hcons x h' => cons (f _ x) (hmap_simple f h')
   end.
 
-Require Import Program.
 
 Lemma nth_member_hget :
   forall A (B : A -> Type) C (f : forall a, B a -> C) c l (h : S.hlist B l) t (m : S.member t l),
@@ -87,14 +72,13 @@ Lemma compile_lift' :
   forall l ty (e : S.expr l ty) ty' n,
     compile (S.lift'(ty' := ty') n e) = U.shift' n (compile e).
 Proof.
-  refine (S.expr_mut_rect' _ _ _ _ _ _); intros; simpl.
+  refine (S.expr_mut_ind' _ _ _ _ _ _); intros; simpl.
   - rewrite member_insert_member.
     break_if; auto.
   - f_equal.
     apply H with (n := (S n)).
   - f_equal; auto.
-  - unfold constr_name.
-    destruct c;
+  - destruct ct;
       repeat destruct args, H as [? args] using S.case_HForall_cons;
       repeat destruct args, H using S.case_HForall_nil;
       simpl; auto using f_equal, f_equal2.
@@ -140,15 +124,14 @@ Theorem compile_subst :
   forall l ty (e : S.expr l ty) l' (h : S.hlist (S.expr l') l),
     compile (S.subst e h) = U.multisubst' (hmap_simple (@compile l') h) (compile e).
 Proof.
-  refine (S.expr_mut_rect' _ _ _ _ _ _); intros; simpl.
+  refine (S.expr_mut_ind' _ _ _ _ _ _); intros; simpl.
   - now rewrite nth_member_hget.
   - f_equal. rewrite H. simpl. f_equal. f_equal.
     rewrite map_hmap_simple, hmap_simple_hmap.
     apply hmap_simple_ext.
     intros. apply compile_lift.
   - f_equal; auto.
-  - unfold constr_name.
-    destruct c;
+  - destruct ct;
       repeat destruct args, H as [? args] using S.case_HForall_cons;
       repeat destruct args, H using S.case_HForall_nil;
       simpl; auto using f_equal, f_equal2.
@@ -164,9 +147,9 @@ Lemma compile_value :
   forall l ty (e : S.expr l ty),
     S.value e -> U.value (compile e).
 Proof.
-  refine (S.expr_mut_rect' _ _ _ _ _ _ ); simpl; intuition.
+  refine (S.expr_mut_ind' _ _ _ _ _ _ ); simpl; intuition.
   constructor.
-  clear c ty.
+  clear c ct ty.
   induction H.
   - auto.
   - intuition.
@@ -179,17 +162,31 @@ Theorem forward_simulation :
     S.step e e' ->
     U.step (compile e) (compile e').
 Proof.
-  intros ty e.
+  intros.
   remember [] as l.
-  revert l ty e Heql.
-  refine (S.expr_mut_rect' _ _ _ _ _ _); simpl; intros; subst; firstorder; subst; simpl.
-  - eauto.
-  - eauto using compile_value.
+  revert Heql.
+  induction H; intros; subst; simpl.
   - rewrite compile_subst. simpl.
     eapply eq_rect.
     constructor. eauto using compile_value.
     unfold U.subst.
     now rewrite U.multisubst'_subst'.
-  - eauto.
+  - auto.
+  - eauto using compile_value.
+  - auto.
+  - match goal with
+    | [ |- context [?f _ _ (S.happ _ _)] ] =>
+      assert (forall l tys1 tys2 (h1 : S.hlist (S.expr l) tys1) (h2 : S.hlist (S.expr l) tys2),
+                 f l (tys1 ++ tys2) (S.happ h1 h2) = f l tys1 h1 ++ f l tys2 h2)
+        as Hfix
+          by (induction h1; simpl; auto using f_equal);
+        rewrite !Hfix; clear Hfix
+    end.
+    apply U.ConstrStep; auto.
+    clear ct.
+    induction args1.
+    + auto.
+    + destruct H using S.case_HForall_hcons.
+      auto using compile_value.
   - admit.
 Admitted.
